code/ecdsap256/Hacl.Impl.P256.Point.fsti
@@ -251,6 +251,14 @@ val aff_point_store: res:lbuffer uint8 64ul -> p:aff_point -> Stack unit
     as_seq h1 res == S.aff_point_store (as_aff_point_nat h0 p))
 
 
+val point_store: res:lbuffer uint8 64ul -> p:point -> Stack unit
+  (requires fun h ->
+    live h res /\ live h p /\ disjoint res p /\
+    point_inv h p)
+  (ensures  fun h0 _ h1 -> modifies (loc res) h0 h1 /\
+    as_seq h1 res == S.point_store (from_mont_point (as_point_nat h0 p)))
+
+
 val load_point_vartime: res:point -> b:lbuffer uint8 64ul -> Stack bool
   (requires fun h ->
     live h res /\ live h b /\ disjoint res b)
